partial/Arith.v
@@ -68,7 +68,7 @@ Qed.
 (** * Calculation *)
 
 (** Boilerplate to import calculation tactics *)
-
+Close Scope memory_scope.
 Module VM <: (Machine mem).
 Definition Conf := Conf.
 Definition Rel := VM.
@@ -81,7 +81,7 @@ Import VMCalc.
 
 (** Specification of the compiler *)
 
-Theorem spec e r a c P : rProp r P -> { s , ⟨comp' e r c, a, s⟩ | P s } =|> {s , ⟨c , eval e, s⟩ | P s } .
+Theorem spec e r c a s : freeFrom r s -> ⟨comp' e r c, a, s⟩  =|> ⟨c , eval e, s⟩ .
 
 
 (** Setup the induction proof *)
@@ -89,7 +89,7 @@ Theorem spec e r a c P : rProp r P -> { s , ⟨comp' e r c, a, s⟩ | P s } =|> 
 Proof.
   intros.
   generalize dependent c.
-  generalize dependent P.
+  generalize dependent s.
   generalize dependent r.
   generalize dependent a.
   induction e;intros.
@@ -99,44 +99,30 @@ Proof.
 (** - [x = Val n]: *)
 
   begin
-    ({s , ⟨ c, eval (Val n), s ⟩ | P s}).
-  ⊇ { auto }
-    ({s , ⟨ c, n, s⟩ | P s}).
+    ⟨c , eval (Val n), s⟩.
+  = {auto}
+      ⟨ c, n, s⟩.
   <== { apply vm_load }
-    ({s , ⟨ LOAD n c, a, s ⟩ | P s}).
-  ⊇ { auto using eqr_refl }
-    ({s , ⟨ LOAD n c, a, s ⟩ | P s}).
+      ⟨ LOAD n c, a, s ⟩.
   [].
 
 (** - [x = Add x1 x2]: *)
   
   begin
-    ({s, ⟨ c, eval (Add e1 e2), s ⟩ | P s}).
-  ⊇ {auto}
-    ({s, ⟨ c, eval e1 + eval e2, s ⟩ | P s}).
-  ⊇ {eauto}
-    ({ s, ⟨c, get r s + eval e2, s⟩ | get r s = eval e1 /\ P s }).
-  <== { apply vm_add}
-    ({ s, ⟨ADD r c, eval e2, s⟩ | get r s = eval e1 /\ P s }).
-  <|= {apply IHe2;eauto}
-   ({ s, ⟨comp' e2 (next r) (ADD r c), eval e1, s⟩ | get r s = eval e1 /\ P s }).
-  ⊇ {try (rewrite <- rProp_set); eauto using get_set}
-    ({s, ⟨comp' e2 (next r) (ADD r c), eval e1, set r (eval e1) s⟩ | P s }).
+    ⟨ c, eval (Add e1 e2), s ⟩.
+  = {auto}
+    ⟨ c, eval e1 + eval e2, s ⟩.
+  ≤ {auto}
+    ⟨c, eval e1 + eval e2, set r (eval e1) s⟩.
+  <== {apply vm_add; eauto using get_set}
+      ⟨ADD r c, eval e2, set r (eval e1) s⟩.
+  <|= {apply IHe2; eauto using freeFrom_set}
+      ⟨comp' e2 (next r) (ADD r c), eval e1, set r (eval e1) s⟩.
   <== { apply vm_store}
-    ({ s, ⟨STORE r (comp' e2 (next r) (ADD r c)), eval e1, s⟩ | P(s) }).
-  <|= { apply IHe1 }
-    ({ s, ⟨comp' e1 r (STORE r (comp' e2 (next r) (ADD r c))), a, s⟩ | P(s) }).
+    ⟨STORE r (comp' e2 (next r) (ADD r c)), eval e1, s⟩.
+  <|= { apply IHe1;eauto }
+    ⟨comp' e1 r (STORE r (comp' e2 (next r) (ADD r c))), a, s⟩.
   [].
-Qed.
-
-
-(* Specialise the spec to singleton sets. *)
-Corollary spec' e r a c s :
-  exists s', ⟨comp' e r c, a, s⟩  =>> ⟨c , eval e, s'⟩ /\ s =[r] s'.
-Proof.
-  pose (spec e r a c (fun s' => s =[r] s')) as S. premise S. eapply rProp_eqr.
-  pose (S (⟨comp' e r c, a, s⟩)) as S'. simpl in S'. premise S'. eexists. split;eauto. 
-  repeat autodestruct; subst; eexists; eauto.
 Qed.
 
 
@@ -148,16 +134,19 @@ Qed.
 
 
 Lemma determ_vm : determ VM.
-  intros C C1 C2 V. induction V; intro V'; inversion V'; subst; reflexivity.
+  intros C C1 C2 V. induction V; intro V'; inversion V'; subst;eauto.
+  rewrite H in *. inversion H5;subst. auto.
 Qed.
 
 
-Theorem sound x a s C : ⟨comp x, a, s⟩ =>>! C -> exists s', C = ⟨HALT, eval x, s'⟩.
+Theorem sound x a s C : freeFrom adr0 s -> ⟨comp x, a, s⟩ =>>! C -> exists s', C = ⟨HALT, eval x, s'⟩.
 Proof.
-  intros.
-  pose (spec' x adr0 a HALT s) as H'. repeat autodestruct. unfold comp in *. pose (determ_trc determ_vm) as D.
-  unfold determ in D. eexists. eapply D. apply H. split. apply H0. intro Contra. destruct Contra.
-  inversion H2.
+  intros F M.
+  pose (spec x adr0 HALT a s F) as H'.
+  destruct H'. destruct H. unfold comp in *. pose (determ_trc determ_vm) as D.
+  unfold determ in D. inversion H0. subst. eexists. eapply D. apply M. split. 
+  apply H. intro Contra. destruct Contra.
+  inversion H1.
 Qed.
 
 End Arith.
